\input{../assets/index.tex}

\begin{document}
    \section*{Matematika 1 cvičení}
    \subsection{Definiční obor}
    \begin{gather*}
        f(a)=\sqrt{\frac{x^2-4x+3}{x+4}}
        \\
            \frac{x^2-4x+3}{x+4} \geq 0 \rightarrow \frac{(x-3)(x-1)}{x+4}
            \\
                D(f)= (-4;1\rangle \cup \langle3;\infty)
            \end{gather*}
    \begin{gather*}
        f(x)=\frac{\ln(x^2-1)}{\ln(x+4)}
        \\
        D(f)=(-4;-3)\cup(-3;-2)\cup(1;\infty)
    \end{gather*}
    \subsection{Grafy funkcí}
    \begin{tabular}{c c c c}
       funkce & $D$ & $H$ & Vlasntnosti \\
       $f(x)=2x-1$ & $D_x = R$ & $H_x = R$ & rostoucí, prostá, spojitá \\\\
       $g(x)=x^2+2x-8$ & $D_x = R$ & $H_x = \langle-9;\infty)$ & -- \\\\
       $h(x)=\frac{(x-1)^5}{32}-1$ & $D_x = R$ & $H_x = R$ & -- \\\\
       $i(x)= \sqrt{2x-4}$ & $D_x = \langle2;\infty)$ & $H_x = \langle0; \infty)$ & -- \\\\
       $j(x)= \frac{3x+3}{3x+1}$ & $D_x= (-\infty;-\frac{1}{3}) \cup (-\frac{1}{3}; \infty)$ & $H_x = (-\infty;1) \cup (1;\infty)$ & --\\\\
       $k(x)= \left( \frac{1}{3}\right)^{x-2}-3$ & $D_x = R$ & $H_y= (-3; \infty)$ & --\\\\
    \end{tabular}
    \subsection*{Limity posloupností}
    \begin{align*}
        \limit{\frac{1}{n}} &= 0
        \\ \limit{a} &= a
        \\ \limit{n} &= \infty
        \\ \limit{(-1)^n} &= neexistuje
        \\ \limit{\left(-\frac{1}{2}\right)^n} &= 0 
        \\ \limit{\frac{3n^2-4n}{1+2n^2}} &= \limit{\frac{(3n^2-4n)\cdot{\frac{1}{n^2}}}{(1+2n^2)\cdot{\frac{1}{n^2}}}} = \limit{\frac{3-\frac{4}{n}}{\frac{1}{n}+2}} =  \doubleunderline{\frac{3}{2}} \\
        \limit{\frac{4n^3-2n-\sqrt{n}}{1-n^2}} &= \limit{\frac{4n-\frac{2}{n}-\frac{1}{\sqrt{n^3}}}{\frac{1}{n^2}-1}} = \left[\frac{\infty}{-1}\right] = \doubleunderline{-\infty} \\
        \limit{\frac{1}{\sqrt{n^2+1}-n}} \cdot \frac{\sqrt{n^2+1}+n}{\sqrt{n^2+1}+n} &= \limit{\frac{\sqrt{n^2+1}+n}{n^2+1-n^2}} = \limit{\frac{\sqrt{n^2+1}+n}{1}} = \limit{\left(\sqrt{n^2+1}+n\right)} = \doubleunderline{\infty} \\
        \limit{\left(\sqrt{2n-1}-\sqrt{2n+3}\right)} \cdot \frac{\sqrt{2n-1}+\sqrt{2n+3}}{\sqrt{2n-1}+\sqrt{2n+3}} &= \frac{-4}{\sqrt{2n-1}+\sqrt{2n+3}} = \doubleunderline{\left[\frac{-4}{\infty}\right]} \\
        \red{\limit{\sqrt[n]{n}}} &= \red{1}  \\
        \red{\limit{\left(1+\frac{1}{2}\right)^n}} &= \red{e} 
    \end{align*}
\end{document}