\input{../assets/index.tex}
\begin{document}
 \section*{Repetitorium matematiky}
\(
(a+b)^2 = a^2 +2ab + b^2 \\
(a-b)^2 = a^2 -2ab + b^2 \\
(a+b)(a-b) = a^2 - b^2
\)
\subsection*{Test repetitorium} 
\begin{example}
    Upravte do základního tvaru: $\left(
        \frac{-16}{3}
    \right) \cdot 
    \sqrt{
        \frac{2}{3}} + 
        \frac{\frac{64}{9}}
        {2\cdot\sqrt{\frac{2}{3}}}$
\end{example}
\begin{gather*}
    \left(
        \frac{-16}{3}
    \right) \cdot 
    \sqrt{
        \frac{2}{3}} + 
        \frac{\frac{64}{9}}
        {2\cdot\sqrt{\frac{2}{3}}} = 
         - \frac{2^4}{3} \cdot \frac{2^\frac{1}{2}}{3^\frac{1}{2}} + \frac{\frac{2^6}{3^2}}{2 \cdot \frac{2^\frac{1}{2}}{3^\frac{1}{2}}} 
        = - \frac{2^\frac{9}{2}}{3^\frac{3}{2}} + \left( \frac{2^6}{3^2} \cdot \frac{3^\frac{1}{2}}{2^\frac{3}{2}} \right)
        = - \frac{2^\frac{9}{2}}{3^\frac{3}{2}} + \frac{2^\frac{9}{2}}{3^\frac{3}{2}} = \doubleunderline{0}
\end{gather*}
\begin{example}
    Zjednodušte $\biggl( x-\frac{3x}{x+1} \biggr)\cdot 
    \biggl( \frac{x-1}{x-2} - \frac{x}{x-1} \biggr) $
\end{example}
\begin{gather*}
    \biggl( x-\frac{3x}{x+1} \biggr)\cdot 
    \biggl( \frac{x-1}{x-2} - \frac{x}{x-1} \biggr) = 
    \biggl( x-\frac{3x}{x+1} \biggr)\cdot 
    \biggl(\frac{x-1}{x-1} \cdot \frac{x-1}{x-2} - \frac{x}{x-1} \biggr) = \\
     = \biggl( x-\frac{3x}{x+1} \biggr)\cdot 
    \biggl( \frac{(x-1)^2}{(x-2)(x-1)} - \frac{x}{x-1} \biggr) = 
    \biggl( x-\frac{3x}{x+1} \biggr)\cdot 
    \biggl( \frac{(x-1)^2 - \bigl(x \cdot (x-2)\bigr)}{(x-2)(x-1)}\biggr) =
    \\  
    = \biggl(\frac{(x+1)x}{x+1} -\frac{3x}{x+1} \biggr)\cdot 
    \biggl( \frac{(x-1)^2 - \bigl(x^2-2x\bigr)}{(x-2)(x-1)}\biggr) =
    \\
    = \biggl(
        \frac{x^2-2x}{x+1} 
    \biggr) \cdot 
    \biggl(
        \frac{x^2-2x+1-x^2+2x}{(x-2)(x-1)}
    \biggr) = \biggl(
        \frac{x^2-2x}{x+1}
    \biggr) \cdot \biggl(
        \frac{1}{(x-2)(x-1)}
    \biggr) = \\=   \frac{x(x-2)}{x+1}  \cdot \frac{1}{(x-2)(x-1)} = \frac{x}{x+1} \cdot \frac{1}{x-1} = \doubleunderline{\frac{x}{x^2-1}}
\end{gather*}
\begin{example}
    Zjednodušte $\frac{3y+2}{y^2-2y+1} - \frac{6}{y^2-1} - \frac{3y-2}{y^2+2y+1}$
\end{example} 
\begin{align*}
    \frac{3y+2}{y^2-2y+1} - \frac{6}{y^2-1} - \frac{3y-2}{y^2+2y+1} 
    \\ &= \frac{3y+2}{(y-1)(y-1)} - \frac{6}{(y+1)(y-1)} - \frac{3y+2}{(y+1)(y+1)} 
    \\ &= \frac{((3y+2)\cdot(y+1))-((6)\cdot(y-1))}{(y-1)^2(y+1)} - \frac{3y+2}{(y+1)^2}
    \\ &= \frac{3y^2+3y+2y+2-6y+6}{(y-1)^2(y+1)} - \frac{3y+2}{(y+1)^2}
    \\ &= \frac{3y^2-y+8}{(y-1)^2(y+1)} - \frac{3y+2}{(y+1)^2}
    \\ &= \frac{((3y^2-y+8)\cdot(y+1))-((3y+2)(y^2-2y+1)}{(y^2-1)^2}
    \\ &= \frac{(3y^3+3y^2-y^2-y+8y+8)-(3y^3-6y^2+3y+2y^2-4y+2)}{(y^2-1)^2}
    \\ &= \frac{3y^3+3y^2-y^2-y+8y+8-3y^3+6y^2-3y-2y^2+4y-2}{(y^2-1)^2}
    \\ &= \frac{6y^2+8y+6}{(y^2-1)^2}
    = \doubleunderline{\frac{2(3y^2+4y+3)}{(y^2-1)^2}}
\end{align*}
\page
\begin{example}
    Řešte rovnici s neznámou $x \in \mathbb{R} $ 
\end{example}
\begin{align*}
    \frac{x+5}{10} - \frac{x-4}{8} &= 1
    \\ \frac{((x+5)\cdot(8)) - ((x-8)\cdot(10))}{80} &= 1
    \\ \frac{8x+40 - 10x +80}{80} &= 1
    \\ 8x + 40 - 10x + 80 &= 80
    \\ -2x  &= -40
    \\   x  &=20
\end{align*}
\page
\subsection*{Hodina 07.10.2022}
 \begin{gather*}
    \biggl( \frac{1}{x+1} - \frac{2x}{x^2-1} \biggr) \biggl(\frac{1}{x} - 1\biggr)
    =  \biggl( \frac{1}{ x+1} - \frac{2x}{(x+1)(x-1)}\biggr)\biggl(\frac{1}{x} -1 \biggr)
    = \\
    = \biggl( \frac{1}{x+1} \frac{x-1}{x-1} - \frac{2x}{(x+1)(x-1)} \biggr)  \biggl(\frac{1}{x}-1\biggr)
    = \biggl( \frac{x-1}{(x+1)(x-1)} - \frac{2x}{(x+1)(x-1)}\biggr) \biggl(\frac{1}{x} - 1\biggr) = 
    \\
    = \biggl(\frac{-x-1}{(x+1)(x-1)}\biggr)\biggl(\frac{1}{x} - \frac{x}{x}\biggr) 
    = \frac{-x-1}{(x+1)(x-1)} \cdot \frac{1 - x}{x}
    = \frac{-(x+1)}{(x+1)(x-1)} \cdot \frac{1-x}{x} =
    \\ = \frac{-1}{x-1} * \frac{1-x}{x} = \frac{-(1-x)}{(x-1)(x)} = \frac{-(-1)(x-1)}{(x-1)x} = \doubleunderline{\frac{1}{x}}
\end{gather*}
\begin{gather*}
    \biggl( \frac{3}{(x-3)^2} + \frac{1}{x+3}- \frac{6}{x^2-9}\biggr) \cdot \frac{x^2-6x+9}{2}
    = \biggl( \frac{3}{(x-3)(x-3)} + \frac{1}{x+3} - \frac{6}{(x+3)(x-3)} \biggr) \cdot \frac{(x-3)(x-3)}{2} =
    \\ = \biggl(
    \frac{3}{(x-3)(x-3)} + \frac{x-3}{(x+3)(x-3)} - \frac{6}{(x+3)(x-3)}
    \biggr) \cdot \frac{(x-3)(x-3)}{2} = \\ = 
    \biggl(
        \frac{3}{(x-3)(x-3)} + \frac{x-9}{(x+3)(x-3)}
    \biggr) \cdot \frac{(x-3)(x-3)}{2} =
    \\ = \biggl(
        \frac{3}{(x-3)(x-3)} + \frac{x-9}{(x+3)(x-3)} \cdot \frac{(x-3)}{(x-3)}
    \biggr) \cdot \frac{(x-3)(x-3)}{2} = \\ =
     \biggl(
        \frac{3}{(x-3)^2} + \frac{(x-9)(x-3)}{(x+3)(x-3)^2} 
    \biggr) \cdot \frac{(x-3)^2}{2} = \frac{3x+9+\bigl((x-9)(x-3)\bigr)}{(x+3)(x-3)^2} \cdot \frac{(x-3)^2}{2} =
    \\ = \frac{3x+9+\bigl((x-9)(x-3)\bigr)}{2(x+3)} = \frac{3x+9+(x^2-3x-9x+27)}{2(x+3)} = \\ =
    \doubleunderline{\frac{x^2-9x+36}{2(x+3)}}
\end{gather*}
\begin{gather*}
    \frac{x^2+7x}{9-x^2} : \frac{x^2-49}{x+3} = \frac{x(x+7)}{(x+3)(-x+3)} \cdot \frac{x+3}{(x+7)(x-7)} = \doubleunderline{\frac{x}{(x-7)(3-x)}}
\end{gather*}
\end{document}
